allow cbor_det_parse_full as a "macro" for C extraction

src/cbor/pulse/CBOR.Pulse.API.Base.fst
@@ -937,3 +937,63 @@ fn map_get_as_option
   }
 }
 ```
+
+module Spec = CBOR.Spec.API.Format
+
+let cbor_det_parse_postcond_some
+  (v: Seq.seq U8.t)
+  (v': Spec.cbor)
+  (vrem: Seq.seq U8.t)
+: Tot prop
+= let s = Spec.cbor_det_serialize v' in
+  let len = Seq.length s in
+  len <= Seq.length v /\
+  Seq.slice v 0 len == s /\
+  Seq.slice v len (Seq.length v) == vrem
+
+noextract [@@noextract_to "krml"]
+let cbor_det_parse_post_some
+  (#cbordet: Type)
+  (cbor_det_match: perm -> cbordet -> Spec.cbor -> slprop)
+  (input: S.slice U8.t)
+  (pm: perm)
+  (v: Seq.seq U8.t)
+  (res: cbordet)
+  (rem: S.slice U8.t)
+: Tot slprop
+= exists* v' vrem .
+     cbor_det_match 1.0R res v' **
+     pts_to rem #pm vrem **
+     Trade.trade // FIXME: I would need a forall_vrem here
+       (cbor_det_match 1.0R res v' ** pts_to rem #pm vrem)
+       (pts_to input #pm v) **
+     pure (
+       cbor_det_parse_postcond_some v v' vrem
+     )
+
+noextract [@@noextract_to "krml"]
+let cbor_det_parse_post
+  (#cbordet: Type)
+  (cbor_det_match: perm -> cbordet -> Spec.cbor -> slprop)
+  (input: S.slice U8.t)
+  (pm: perm)
+  (v: Seq.seq U8.t)
+  (res: option (cbordet & S.slice U8.t))
+: Tot slprop
+= match res with
+  | None -> pts_to input #pm v ** pure (~ (exists v1 v2 . v == Spec.cbor_det_serialize v1 `Seq.append` v2))
+  | Some (res, rem) -> cbor_det_parse_post_some cbor_det_match input pm v res rem
+
+inline_for_extraction
+let cbor_det_parse_t
+  (#cbordet: Type)
+  (cbor_det_match: perm -> cbordet -> Spec.cbor -> slprop)
+=
+  (input: S.slice U8.t) ->
+  (#pm: perm) ->
+  (#v: Ghost.erased (Seq.seq U8.t)) ->
+  stt (option (cbordet & S.slice U8.t))
+    (pts_to input #pm v)
+    (fun res ->
+      cbor_det_parse_post cbor_det_match input pm v res
+    )
