src/cbor/pulse/CBOR.Pulse.API.Det.C.Slice.fst
@@ -1,0 +1,93 @@
+module CBOR.Pulse.API.Det.C.Slice
+#lang-pulse
+include CBOR.Pulse.API.Det.C
+open Pulse.Lib.Pervasives
+open CBOR.Spec.Constants
+
+module Spec = CBOR.Spec.API.Format
+module S = Pulse.Lib.Slice
+module A = Pulse.Lib.Array
+module PM = Pulse.Lib.SeqMatch
+module Trade = Pulse.Lib.Trade.Util
+module SZ = FStar.SizeT
+module U64 = FStar.UInt64
+module U8 = FStar.UInt8
+
+module SU = Pulse.Lib.Slice.Util
+module AP = Pulse.Lib.ArrayPtr
+
+inline_for_extraction noextract [@@noextract_to "krml"]
+fn cbor_det_validate_from_slice
+  (_: unit)
+: cbor_det_validate_t
+=
+  (input: S.slice U8.t)
+  (#pm: perm)
+  (#v: Ghost.erased (Seq.seq U8.t))
+{
+  S.pts_to_len input;
+  let len = S.len input;
+  let a = SU.slice_to_arrayptr_intro_trade input;
+  let res = cbor_det_validate a len;
+  Trade.elim _ _;
+  res
+}
+
+inline_for_extraction
+noextract [@@noextract_to "krml"]
+fn cbor_det_parse_from_slice
+  (input: S.slice U8.t) // the length of that slice does not really matter
+  (len: SZ.t)
+  (#pm: perm)
+  (#v: Ghost.erased (Seq.seq U8.t))
+requires
+    (pts_to input #pm v ** pure (
+      exists v1 v2 . Ghost.reveal v == Spec.cbor_det_serialize v1 `Seq.append` v2 /\ SZ.v len == Seq.length (Spec.cbor_det_serialize v1)
+    ))
+returns res: cbor_det_t
+ensures
+    (exists* v' .
+      cbor_det_match 1.0R res v' **
+      Trade.trade (cbor_det_match 1.0R res v') (pts_to input #pm v) ** pure (
+        SZ.v len <= Seq.length v /\
+        Seq.slice v 0 (SZ.v len) == Spec.cbor_det_serialize v'
+    ))
+{
+  S.pts_to_len input;
+  let a = SU.slice_to_arrayptr_intro_trade input;
+  let res = cbor_det_parse a len;
+  Trade.trans _ _ (pts_to input #pm v);
+  res
+}
+
+inline_for_extraction
+noextract [@@noextract_to "krml"]
+fn cbor_det_parse_valid
+  (_: unit)
+: cbor_det_parse_valid_t
+=
+  (input: S.slice U8.t)
+  (#pm: perm)
+  (#v: Ghost.erased (Seq.seq U8.t))
+{
+  let len = S.len input;
+  S.pts_to_len input;
+  Classical.forall_intro cbor_det_parse_aux1;
+  let a = SU.slice_to_arrayptr_intro_trade input;
+  let res = cbor_det_parse a len;
+  Trade.trans _ _ (pts_to input #pm v);
+  res
+}
+
+inline_for_extraction
+noextract [@@noextract_to "krml"]
+fn cbor_det_parse_full
+  (_: unit)
+: cbor_det_parse_t u#0 #_ cbor_det_match
+= (input: _)
+  (#pm: _)
+  (#v: _)
+{
+  CBOR.Pulse.API.Det.Common.cbor_det_parse_full (cbor_det_validate_from_slice ()) (cbor_det_parse_valid ())
+    input
+}
